src/Lib/Callback/Overrun.v
@@ -15,7 +15,7 @@ Definition callback  : funspec :=
          size : Z,
          key_p : val, 
          (* overrun_encoder_key fields *)
-         buf_p : val,
+         buf_b : block, buf_ofs : ptrofs, 
          buf_size : Z, computed_size : Z
     PRE [tptr tvoid, tuint, tptr tvoid]
       PROP (size = Zlength data;
@@ -23,29 +23,35 @@ Definition callback  : funspec :=
             0 <= computed_size <= Int.max_unsigned;
             0 <= size <= Int.max_unsigned;
             0 <= computed_size + size <= Int.max_unsigned;
-            isptr buf_p;
-            if buf_size <? computed_size + size 
-            then buf_size = 0 else True)
+            0 <= computed_size + size + Ptrofs.unsigned buf_ofs < Ptrofs.modulus;
+            0 <= Ptrofs.unsigned buf_ofs + buf_size < Ptrofs.modulus)
       PARAMS (data_p; Vint (Int.repr size); key_p)
       GLOBALS ()
       SEP (data_at Tsh (tarray tuchar (Zlength data)) (map Vint data) data_p;
            data_at Tsh enc_key_s 
-                   (mk_enc_key buf_p buf_size computed_size)
+                   (mk_enc_key (Vptr buf_b buf_ofs) buf_size computed_size)
                    key_p;
-          if buf_size <? computed_size + size
-          then emp
-          else memory_block Tsh size (offset_val computed_size buf_p))
+            memory_block Tsh buf_size  (Vptr buf_b buf_ofs))
      POST [tint]
       PROP ()
       LOCAL (temp ret_temp Vzero)
       SEP (data_at Tsh (tarray tuchar (Zlength data)) (map Vint data) data_p;
            if buf_size <? computed_size + size 
-           then data_at Tsh enc_key_s (mk_enc_key buf_p 0
-                                                  (computed_size + size)) key_p
-           else (data_at Tsh (tarray tuchar size) (map Vint data) 
-                         (offset_val computed_size buf_p) * 
-                 data_at Tsh enc_key_s (mk_enc_key buf_p buf_size 
-                                                   (computed_size + size)) key_p)). 
+           then 
+             (data_at Tsh enc_key_s
+                      (mk_enc_key 
+                         (Vptr buf_b buf_ofs) 0 (computed_size + size)) key_p *
+                memory_block Tsh buf_size  (Vptr buf_b buf_ofs))
+           else 
+             (memory_block Tsh computed_size (Vptr buf_b buf_ofs)*
+              data_at Tsh (tarray tuchar size) (map Vint data) 
+                      (offset_val computed_size (Vptr buf_b buf_ofs)) * 
+              memory_block Tsh (buf_size - computed_size - len data)
+                           (offset_val (computed_size + len data) 
+                                       (Vptr buf_b buf_ofs)) *
+              data_at Tsh enc_key_s 
+                      (mk_enc_key  (Vptr buf_b buf_ofs) buf_size 
+                                   (computed_size + size)) key_p)). 
 
 Definition callback_overrun_spec : ident * funspec :=
   DECLARE _overrun_encoder_cb callback.
@@ -58,20 +64,22 @@ Theorem bool_der_encode : semax_body Vprog Gprog f_overrun_encoder_cb
                                      callback_overrun_spec.
 Proof.
   start_function.
+  remember  (Vptr buf_b buf_ofs) as buf_p.
   destruct (buf_size <? computed_size + size) eqn:S.
   - repeat forward. 
     assert (buf_size < computed_size + size) by (Zbool_to_Prop; eassumption).
     forward_if 
       (PROP ()
-       LOCAL (temp _t'3 (Vint (Int.repr 0)); 
+       LOCAL (temp _t'3 (Vint (Int.repr buf_size)); 
               temp _t'2 (Vint (Int.repr computed_size));
               temp _key key_p; temp _data data_p; 
               temp _size (Vint (Int.repr size));
               temp _keyp key_p)
        SEP (data_at Tsh (tarray tuchar (Zlength data)) (map Vint data) data_p;
             data_at Tsh enc_key_s 
-                    (mk_enc_key buf_p 0 computed_size) key_p));
-      repeat (forward || entailer! || nia).    
+                    (mk_enc_key buf_p 0 computed_size) key_p;
+      memory_block Tsh buf_size buf_p));
+    repeat (forward || entailer! || nia). 
   - assert (computed_size + size <= buf_size) by (Zbool_to_Prop; eassumption).
     repeat forward.
     unfold mk_enc_key.
@@ -89,9 +97,23 @@ Proof.
                  data_at Tsh (tarray tuchar size) (map Vint data) 
                          (offset_val computed_size buf_p);
                  data_at Tsh enc_key_s 
-                         (mk_enc_key buf_p buf_size (computed_size)) key_p));
+                         (mk_enc_key buf_p buf_size (computed_size)) key_p; 
+       (memory_block Tsh computed_size buf_p) ;
+                memory_block Tsh (buf_size - computed_size - len data)
+                             (offset_val (computed_size + len data) buf_p))) ;
       repeat (forward || entailer! || nia). 
     forward_call (Tsh, Tsh, offset_val computed_size buf_p, data_p, size, data);
       entailer!.
+    cbn; entailer!.
+    replace buf_size with ((computed_size + len data)
+                           + (buf_size - computed_size - len data)) at 1 by nia.
+    unfold offset_val.
+    replace buf_ofs with (Ptrofs.repr (Ptrofs.unsigned buf_ofs)).
+    erewrite memory_block_split.
+    erewrite memory_block_split.
+    entailer!.
+    all: try nia; rep_omega_setup;
+    try rep_omega.
+    rewrite Ptrofs.repr_unsigned; auto.
     cbn; entailer!.
 Qed.
